examples/ghc/module-edits/SrcLoc/midamble.v
@@ -1,3 +1,22 @@
 (* Default values *)
 Require Import GHC.Err.
 Instance Default__SrcSpan : Default SrcSpan := Build_Default _ (UnhelpfulSpan default).
+
+Instance Default__RealSrcSpan : Default RealSrcSpan := 
+  Build_Default _ (RealSrcSpan' GHC.Err.default GHC.Err.default  GHC.Err.default  
+                   GHC.Err.default GHC.Err.default).
+
+Definition Ord__RealSrcLoc_op_zl : RealSrcLoc -> RealSrcLoc -> bool :=
+  fun a b =>
+    let 'ASrcLoc a1 a2 a3 := a in
+    let 'ASrcLoc b1 b2 b3 := b in
+    match (GHC.Base.compare a1 b1) with
+    | Lt => true
+    | Eq =>
+        match (GHC.Base.compare a2 b2) with
+        | Lt => true
+        | Eq => (a3 GHC.Base.< b3)
+        | Gt => false
+        end
+    | Gt => false
+    end.
