examples/ghc/lib/CoreFVs.v
@@ -18,10 +18,19 @@ Require Import CoreSyn.
 
 Require BasicTypes.
 Require CoreSyn.
+Require Data.Foldable.
+Require Data.Tuple.
 Require FV.
+Require GHC.Base.
+Require GHC.DeferredFix.
+Require GHC.List.
+Require Lists.List.
 Require NameSet.
+Require UniqSet.
+Require Unique.
 Require Var.
 Require VarSet.
+Import GHC.Base.Notations.
 
 (* Converted type declarations: *)
 
@@ -41,170 +50,395 @@ Definition CoreAltWithFVs :=
   (AnnAlt Var.Id FVAnn)%type.
 (* Midamble *)
 
+(* Break mutual recursion *)
+Parameter rhs_fvs1 : (Var.Id * CoreSyn.CoreExpr)%type -> FV.FV.
+
+(* Break mutual recursion *)
+Parameter freeVarsBind1 : CoreSyn.CoreBind ->
+     VarSet.DVarSet -> (CoreBindWithFVs * VarSet.DVarSet)%type.
+
+(*
+NOTE (freeVars): if you try to use a termination edit for freeVars instead of 
+the rewrite of unzipAndMap in the edit file, we need to add a type
+annotation to fv_alt for the freeVars function to type check. 
+The required annotation is 
+   fv_alt : Alt CoreBndr -> (VarSet.DVarSet * CoreAltWithFVs)
+*)
 
 (* Converted value declarations: *)
 
-Axiom exprFreeVars : CoreSyn.CoreExpr -> VarSet.VarSet.
-
-Axiom exprsFreeVarsList : list CoreSyn.CoreExpr -> list Var.Var.
-
-Axiom exprsFreeVars : list CoreSyn.CoreExpr -> VarSet.VarSet.
-
-Axiom exprsFVs : list CoreSyn.CoreExpr -> FV.FV.
-
-Axiom exprFreeVarsList : CoreSyn.CoreExpr -> list Var.Var.
-
-Axiom exprFreeVarsDSet : CoreSyn.CoreExpr -> VarSet.DVarSet.
-
-Axiom exprFVs : CoreSyn.CoreExpr -> FV.FV.
-
-Axiom exprFreeIds : CoreSyn.CoreExpr -> VarSet.IdSet.
-
-Axiom exprFreeIdsDSet : CoreSyn.CoreExpr -> VarSet.DIdSet.
-
-Axiom exprFreeIdsList : CoreSyn.CoreExpr -> list Var.Id.
-
-Axiom exprsFreeIdsDSet : list CoreSyn.CoreExpr -> VarSet.DIdSet.
-
-Axiom exprsFreeIdsList : list CoreSyn.CoreExpr -> list Var.Id.
-
-Axiom bindFreeVars : CoreSyn.CoreBind -> VarSet.VarSet.
-
-Axiom exprSomeFreeVars : FV.InterestingVarFun ->
-                         CoreSyn.CoreExpr -> VarSet.VarSet.
-
-Axiom exprSomeFreeVarsList : FV.InterestingVarFun ->
-                             CoreSyn.CoreExpr -> list Var.Var.
-
-Axiom exprSomeFreeVarsDSet : FV.InterestingVarFun ->
-                             CoreSyn.CoreExpr -> VarSet.DVarSet.
-
-Axiom exprsSomeFreeVars : FV.InterestingVarFun ->
-                          list CoreSyn.CoreExpr -> VarSet.VarSet.
-
-Axiom exprsSomeFreeVarsList : FV.InterestingVarFun ->
-                              list CoreSyn.CoreExpr -> list Var.Var.
-
-Axiom exprsSomeFreeVarsDSet : FV.InterestingVarFun ->
-                              list CoreSyn.CoreExpr -> VarSet.DVarSet.
-
-Axiom stableUnfoldingVars : CoreSyn.Unfolding -> option VarSet.VarSet.
-
-Axiom idUnfoldingVars : Var.Id -> VarSet.VarSet.
-
-Axiom freeVars : CoreSyn.CoreExpr -> CoreExprWithFVs.
-
-Axiom freeVarsBind : CoreSyn.CoreBind ->
-                     VarSet.DVarSet -> (CoreBindWithFVs * VarSet.DVarSet)%type.
-
-Axiom bndrRuleAndUnfoldingVarsDSet : Var.Id -> VarSet.DVarSet.
-
-Axiom dIdFreeVars : Var.Id -> VarSet.DVarSet.
-
-Axiom idFreeVars : Var.Id -> VarSet.VarSet.
-
-Axiom idFVs : Var.Id -> FV.FV.
-
-Axiom vectsFreeVars : list CoreSyn.CoreVect -> VarSet.VarSet.
-
-Axiom idRuleRhsVars : (BasicTypes.Activation -> bool) ->
-                      Var.Id -> VarSet.VarSet.
-
-Axiom ruleRhsFreeVars : CoreSyn.CoreRule -> VarSet.VarSet.
-
-Axiom ruleLhsFreeIdsList : CoreSyn.CoreRule -> list Var.Var.
-
-Axiom ruleLhsFreeIds : CoreSyn.CoreRule -> VarSet.VarSet.
-
-Axiom ruleLhsFVIds : CoreSyn.CoreRule -> FV.FV.
-
-Axiom rulesFreeVarsDSet : list CoreSyn.CoreRule -> VarSet.DVarSet.
-
-Axiom rulesFVs : list CoreSyn.CoreRule -> FV.FV.
-
-Axiom rulesFreeVars : list CoreSyn.CoreRule -> VarSet.VarSet.
-
-Axiom ruleFreeVars : CoreSyn.CoreRule -> VarSet.VarSet.
-
-Axiom ruleFVs : CoreSyn.CoreRule -> FV.FV.
-
-Axiom exprs_fvs : list CoreSyn.CoreExpr -> FV.FV.
-
-Axiom stableUnfoldingFVs : CoreSyn.Unfolding -> option FV.FV.
-
-Axiom idUnfoldingFVs : Var.Id -> FV.FV.
-
-Axiom bndrRuleAndUnfoldingFVs : Var.Id -> FV.FV.
-
-Axiom rhs_fvs : (Var.Id * CoreSyn.CoreExpr)%type -> FV.FV.
-
-Axiom expr_fvs : CoreSyn.CoreExpr -> FV.FV.
-
-Axiom addBndrs : list CoreSyn.CoreBndr -> FV.FV -> FV.FV.
-
-Axiom addBndr : CoreSyn.CoreBndr -> FV.FV -> FV.FV.
-
-(* tickish_fvs skipped *)
-
-(* exprsOrphNames skipped *)
-
-(* exprOrphNames skipped *)
-
-(* orphNamesOfFamInst skipped *)
-
-(* orphNamesOfAxiom skipped *)
-
-(* orphNamesOfCos skipped *)
-
-(* orphNamesOfProv skipped *)
-
-(* orphNamesOfCo skipped *)
-
-(* orphNamesOfTypes skipped *)
-
-(* orphNamesOfType skipped *)
-
-(* orphNamesOfCoAxBranch skipped *)
-
-(* orphNamesOfCoAxBranches skipped *)
-
-(* orphNamesOfCoCon skipped *)
-
-(* orphNamesOfTyCon skipped *)
-
-Axiom orphNamesOfThings : forall {a},
-                          (a -> NameSet.NameSet) -> list a -> NameSet.NameSet.
-
-Axiom freeVarsOf : CoreExprWithFVs -> VarSet.DIdSet.
-
-Axiom freeVarsOfAnn : FVAnn -> VarSet.DIdSet.
-
-Axiom noFVs : VarSet.VarSet.
-
-Axiom aFreeVar : Var.Var -> VarSet.DVarSet.
-
-Axiom delBindersFV : list Var.Var -> VarSet.DVarSet -> VarSet.DVarSet.
-
-Axiom delBinderFV : Var.Var -> VarSet.DVarSet -> VarSet.DVarSet.
-
-Axiom unionFVs : VarSet.DVarSet -> VarSet.DVarSet -> VarSet.DVarSet.
-
-Axiom unionFVss : list VarSet.DVarSet -> VarSet.DVarSet.
-
-(* varTypeTyCoVars skipped *)
-
-(* dVarTypeTyCoVars skipped *)
-
-(* varTypeTyCoFVs skipped *)
-
-Axiom idRuleVars : Var.Id -> VarSet.VarSet.
-
-Axiom idRuleFVs : Var.Id -> FV.FV.
+Definition aFreeVar : Var.Var -> VarSet.DVarSet :=
+  VarSet.unitDVarSet.
+
+Definition freeVarsOf : CoreExprWithFVs -> VarSet.DIdSet :=
+  fun '(pair fvs _) => fvs.
+
+Definition freeVarsOfAnn : FVAnn -> VarSet.DIdSet :=
+  fun fvs => fvs.
+
+Definition idRuleFVs : Var.Id -> FV.FV :=
+  fun id => FV.emptyFV.
+
+Definition idRuleVars : Var.Id -> VarSet.VarSet :=
+  fun id => FV.fvVarSet (idRuleFVs id).
+
+Definition idUnfoldingFVs : Var.Id -> FV.FV :=
+  fun id => FV.emptyFV.
+
+Definition idUnfoldingVars : Var.Id -> VarSet.VarSet :=
+  fun id => FV.fvVarSet (idUnfoldingFVs id).
+
+Definition bndrRuleAndUnfoldingFVs : Var.Id -> FV.FV :=
+  fun id =>
+    if Var.isId id : bool then FV.unionFV (idRuleFVs id) (idUnfoldingFVs id) else
+    FV.emptyFV.
+
+Definition bndrRuleAndUnfoldingVarsDSet : Var.Id -> VarSet.DVarSet :=
+  fun id => FV.fvDVarSet (bndrRuleAndUnfoldingFVs id).
+
+Definition noFVs : VarSet.VarSet :=
+  VarSet.emptyVarSet.
+
+Definition orphNamesOfThings {a}
+   : (a -> NameSet.NameSet) -> list a -> NameSet.NameSet :=
+  fun f =>
+    Data.Foldable.foldr (NameSet.unionNameSet GHC.Base.∘ f) NameSet.emptyNameSet.
+
+Definition tickish_fvs : CoreSyn.Tickish Var.Id -> FV.FV :=
+  fun arg_0__ =>
+    match arg_0__ with
+    | CoreSyn.Breakpoint _ ids => FV.mkFVs ids
+    | _ => FV.emptyFV
+    end.
+
+Definition unionFVs : VarSet.DVarSet -> VarSet.DVarSet -> VarSet.DVarSet :=
+  VarSet.unionDVarSet.
+
+Definition unionFVss : list VarSet.DVarSet -> VarSet.DVarSet :=
+  VarSet.unionDVarSets.
+
+Definition varTypeTyCoFVs : Var.Var -> FV.FV :=
+  fun var => FV.emptyFV.
+
+Definition varTypeTyCoVars : Var.Var -> VarSet.TyCoVarSet :=
+  fun var => FV.fvVarSet (varTypeTyCoFVs var).
+
+Definition dVarTypeTyCoVars : Var.Var -> VarSet.DTyCoVarSet :=
+  fun var => FV.fvDVarSet (varTypeTyCoFVs var).
+
+Definition delBinderFV : Var.Var -> VarSet.DVarSet -> VarSet.DVarSet :=
+  fun b s => unionFVs (VarSet.delDVarSet s b) (dVarTypeTyCoVars b).
+
+Definition delBindersFV : list Var.Var -> VarSet.DVarSet -> VarSet.DVarSet :=
+  fun bs fvs => Data.Foldable.foldr delBinderFV fvs bs.
+
+Definition freeVars : CoreSyn.CoreExpr -> CoreExprWithFVs :=
+  let go : CoreSyn.CoreExpr -> CoreExprWithFVs :=
+    fix go arg_0__
+          := match arg_0__ with
+             | CoreSyn.Var v =>
+                 let ty_fvs := dVarTypeTyCoVars v in
+                 if Var.isLocalVar v : bool
+                 then pair (unionFVs (aFreeVar v) ty_fvs) (CoreSyn.AnnVar v) else
+                 pair VarSet.emptyDVarSet (CoreSyn.AnnVar v)
+             | CoreSyn.Lit lit => pair VarSet.emptyDVarSet (CoreSyn.AnnLit lit)
+             | CoreSyn.Lam b body =>
+                 let b_ty := tt in
+                 let b_fvs := VarSet.emptyDVarSet in
+                 let '(pair body_fvs _ as body') := go body in
+                 pair (unionFVs b_fvs (delBinderFV b body_fvs)) (CoreSyn.AnnLam b body')
+             | CoreSyn.App fun_ arg =>
+                 let arg' := go arg in
+                 let fun' := go fun_ in
+                 pair (unionFVs (freeVarsOf fun') (freeVarsOf arg')) (CoreSyn.AnnApp fun' arg')
+             | CoreSyn.Case scrut bndr ty alts =>
+                 let fv_alt :=
+                   fun '(pair (pair con args) rhs) =>
+                     let rhs2 := go rhs in
+                     pair (delBindersFV args (freeVarsOf rhs2)) (pair (pair con args) rhs2) in
+                 let 'pair alts_fvs_s alts2 := GHC.List.unzip (Lists.List.map fv_alt alts) in
+                 let alts_fvs := unionFVss alts_fvs_s in
+                 let scrut2 := go scrut in
+                 pair (unionFVs (unionFVs (delBinderFV bndr alts_fvs) (freeVarsOf scrut2))
+                                VarSet.emptyDVarSet) (CoreSyn.AnnCase scrut2 bndr ty alts2)
+             | CoreSyn.Let bind body =>
+                 let body2 := go body in
+                 let 'pair bind2 bind_fvs := freeVarsBind1 bind (freeVarsOf body2) in
+                 pair bind_fvs (CoreSyn.AnnLet bind2 body2)
+             | CoreSyn.Cast expr co =>
+                 let cfvs := VarSet.emptyDVarSet in
+                 let expr2 := go expr in
+                 pair (unionFVs (freeVarsOf expr2) cfvs) (CoreSyn.AnnCast expr2 (pair cfvs co))
+             | CoreSyn.Tick tickish expr =>
+                 let tickishFVs :=
+                   fun arg_23__ =>
+                     match arg_23__ with
+                     | CoreSyn.Breakpoint _ ids => VarSet.mkDVarSet ids
+                     | _ => VarSet.emptyDVarSet
+                     end in
+                 let expr2 := go expr in
+                 pair (unionFVs (tickishFVs tickish) (freeVarsOf expr2)) (CoreSyn.AnnTick tickish
+                       expr2)
+             | CoreSyn.Type_ ty => pair VarSet.emptyDVarSet (CoreSyn.AnnType ty)
+             | CoreSyn.Coercion co => pair VarSet.emptyDVarSet (CoreSyn.AnnCoercion co)
+             end in
+  go.
+
+Definition freeVarsBind
+   : CoreSyn.CoreBind ->
+     VarSet.DVarSet -> (CoreBindWithFVs * VarSet.DVarSet)%type :=
+  fun arg_0__ arg_1__ =>
+    match arg_0__, arg_1__ with
+    | CoreSyn.NonRec binder rhs, body_fvs =>
+        let body_fvs2 := delBinderFV binder body_fvs in
+        let rhs2 := freeVars rhs in
+        pair (CoreSyn.AnnNonRec binder rhs2) (unionFVs (unionFVs (freeVarsOf rhs2)
+                                                                 body_fvs2) (bndrRuleAndUnfoldingVarsDSet binder))
+    | CoreSyn.Rec binds, body_fvs =>
+        let 'pair binders rhss := GHC.List.unzip binds in
+        let rhss2 := GHC.Base.map freeVars rhss in
+        let rhs_body_fvs :=
+          Data.Foldable.foldr (unionFVs GHC.Base.∘ freeVarsOf) body_fvs rhss2 in
+        let binders_fvs :=
+          FV.fvDVarSet (FV.mapUnionFV bndrRuleAndUnfoldingFVs binders) in
+        let all_fvs := unionFVs rhs_body_fvs binders_fvs in
+        pair (CoreSyn.AnnRec (GHC.List.zip binders rhss2)) (delBindersFV binders
+              all_fvs)
+    end.
+
+Definition idFVs : Var.Id -> FV.FV :=
+  fun id => FV.unionFV (varTypeTyCoFVs id) (bndrRuleAndUnfoldingFVs id).
+
+Definition dIdFreeVars : Var.Id -> VarSet.DVarSet :=
+  fun id => FV.fvDVarSet (idFVs id).
+
+Definition idFreeVars : Var.Id -> VarSet.VarSet :=
+  fun id => FV.fvVarSet (idFVs id).
+
+Definition addBndr : CoreSyn.CoreBndr -> FV.FV -> FV.FV :=
+  fun bndr fv fv_cand in_scope acc =>
+    (FV.unionFV (varTypeTyCoFVs bndr) (FV.delFV bndr fv)) fv_cand in_scope acc.
+
+Definition addBndrs : list CoreSyn.CoreBndr -> FV.FV -> FV.FV :=
+  fun bndrs fv => Data.Foldable.foldr addBndr fv bndrs.
+
+Definition expr_fvs : CoreSyn.CoreExpr -> FV.FV :=
+  GHC.DeferredFix.deferredFix4 (fun expr_fvs arg_0__ arg_1__ arg_2__ arg_3__ =>
+                                  match arg_0__, arg_1__, arg_2__, arg_3__ with
+                                  | CoreSyn.Type_ ty, fv_cand, in_scope, acc => FV.emptyFV fv_cand in_scope acc
+                                  | CoreSyn.Coercion co, fv_cand, in_scope, acc => FV.emptyFV fv_cand in_scope acc
+                                  | CoreSyn.Var var, fv_cand, in_scope, acc => FV.unitFV var fv_cand in_scope acc
+                                  | CoreSyn.Lit _, fv_cand, in_scope, acc => FV.emptyFV fv_cand in_scope acc
+                                  | CoreSyn.Tick t expr, fv_cand, in_scope, acc =>
+                                      (FV.unionFV (tickish_fvs t) (expr_fvs expr)) fv_cand in_scope acc
+                                  | CoreSyn.App fun_ arg, fv_cand, in_scope, acc =>
+                                      (FV.unionFV (expr_fvs fun_) (expr_fvs arg)) fv_cand in_scope acc
+                                  | CoreSyn.Lam bndr body, fv_cand, in_scope, acc =>
+                                      addBndr bndr (expr_fvs body) fv_cand in_scope acc
+                                  | CoreSyn.Cast expr co, fv_cand, in_scope, acc =>
+                                      (FV.unionFV (expr_fvs expr) FV.emptyFV) fv_cand in_scope acc
+                                  | CoreSyn.Case scrut bndr ty alts, fv_cand, in_scope, acc =>
+                                      let alt_fvs :=
+                                        fun '(pair (pair _ bndrs) rhs) => addBndrs bndrs (expr_fvs rhs) in
+                                      (FV.unionFV (FV.unionFV (expr_fvs scrut) FV.emptyFV) (addBndr bndr
+                                                   (FV.mapUnionFV alt_fvs alts))) fv_cand in_scope acc
+                                  | CoreSyn.Let (CoreSyn.NonRec bndr rhs) body, fv_cand, in_scope, acc =>
+                                      (FV.unionFV (rhs_fvs1 (pair bndr rhs)) (addBndr bndr (expr_fvs body))) fv_cand
+                                      in_scope acc
+                                  | CoreSyn.Let (CoreSyn.Rec pairs) body, fv_cand, in_scope, acc =>
+                                      addBndrs (GHC.Base.map Data.Tuple.fst pairs) (FV.unionFV (FV.mapUnionFV rhs_fvs1
+                                                                                                pairs) (expr_fvs body))
+                                      fv_cand in_scope acc
+                                  end).
+
+Definition exprFVs : CoreSyn.CoreExpr -> FV.FV :=
+  FV.filterFV Var.isLocalVar GHC.Base.∘ expr_fvs.
+
+Definition exprFreeVars : CoreSyn.CoreExpr -> VarSet.VarSet :=
+  FV.fvVarSet GHC.Base.∘ exprFVs.
+
+Definition exprFreeVarsDSet : CoreSyn.CoreExpr -> VarSet.DVarSet :=
+  FV.fvDVarSet GHC.Base.∘ exprFVs.
+
+Definition exprFreeVarsList : CoreSyn.CoreExpr -> list Var.Var :=
+  FV.fvVarList GHC.Base.∘ exprFVs.
+
+Definition exprsFVs : list CoreSyn.CoreExpr -> FV.FV :=
+  fun exprs => FV.mapUnionFV exprFVs exprs.
+
+Definition exprsFreeVars : list CoreSyn.CoreExpr -> VarSet.VarSet :=
+  FV.fvVarSet GHC.Base.∘ exprsFVs.
+
+Definition exprsFreeVarsList : list CoreSyn.CoreExpr -> list Var.Var :=
+  FV.fvVarList GHC.Base.∘ exprsFVs.
+
+Definition exprSomeFreeVars
+   : FV.InterestingVarFun -> CoreSyn.CoreExpr -> VarSet.VarSet :=
+  fun fv_cand e => FV.fvVarSet (FV.filterFV fv_cand (expr_fvs e)).
+
+Definition exprFreeIds : CoreSyn.CoreExpr -> VarSet.IdSet :=
+  exprSomeFreeVars Var.isLocalId.
+
+Definition exprSomeFreeVarsDSet
+   : FV.InterestingVarFun -> CoreSyn.CoreExpr -> VarSet.DVarSet :=
+  fun fv_cand e => FV.fvDVarSet (FV.filterFV fv_cand (expr_fvs e)).
+
+Definition exprFreeIdsDSet : CoreSyn.CoreExpr -> VarSet.DIdSet :=
+  exprSomeFreeVarsDSet Var.isLocalId.
+
+Definition exprSomeFreeVarsList
+   : FV.InterestingVarFun -> CoreSyn.CoreExpr -> list Var.Var :=
+  fun fv_cand e => FV.fvVarList (FV.filterFV fv_cand (expr_fvs e)).
+
+Definition exprFreeIdsList : CoreSyn.CoreExpr -> list Var.Id :=
+  exprSomeFreeVarsList Var.isLocalId.
+
+Definition exprsSomeFreeVars
+   : FV.InterestingVarFun -> list CoreSyn.CoreExpr -> VarSet.VarSet :=
+  fun fv_cand es => FV.fvVarSet (FV.filterFV fv_cand (FV.mapUnionFV expr_fvs es)).
+
+Definition exprsSomeFreeVarsDSet
+   : FV.InterestingVarFun -> list CoreSyn.CoreExpr -> VarSet.DVarSet :=
+  fun fv_cand e => FV.fvDVarSet (FV.filterFV fv_cand (FV.mapUnionFV expr_fvs e)).
+
+Definition exprsFreeIdsDSet : list CoreSyn.CoreExpr -> VarSet.DIdSet :=
+  exprsSomeFreeVarsDSet Var.isLocalId.
+
+Definition exprsSomeFreeVarsList
+   : FV.InterestingVarFun -> list CoreSyn.CoreExpr -> list Var.Var :=
+  fun fv_cand es =>
+    FV.fvVarList (FV.filterFV fv_cand (FV.mapUnionFV expr_fvs es)).
+
+Definition exprsFreeIdsList : list CoreSyn.CoreExpr -> list Var.Id :=
+  exprsSomeFreeVarsList Var.isLocalId.
+
+Definition exprs_fvs : list CoreSyn.CoreExpr -> FV.FV :=
+  fun exprs => FV.mapUnionFV expr_fvs exprs.
+
+Definition ruleFVs : CoreSyn.CoreRule -> FV.FV :=
+  fun arg_0__ =>
+    match arg_0__ with
+    | CoreSyn.BuiltinRule _ _ _ _ => FV.emptyFV
+    | CoreSyn.Rule _ _ _do_not_include _ bndrs args rhs _ _ _ _ =>
+        FV.filterFV Var.isLocalVar (addBndrs bndrs (exprs_fvs (cons rhs args)))
+    end.
+
+Definition ruleFreeVars : CoreSyn.CoreRule -> VarSet.VarSet :=
+  FV.fvVarSet GHC.Base.∘ ruleFVs.
+
+Definition rulesFreeVars : list CoreSyn.CoreRule -> VarSet.VarSet :=
+  fun rules => VarSet.mapUnionVarSet ruleFreeVars rules.
+
+Definition rulesFVs : list CoreSyn.CoreRule -> FV.FV :=
+  FV.mapUnionFV ruleFVs.
+
+Definition rulesFreeVarsDSet : list CoreSyn.CoreRule -> VarSet.DVarSet :=
+  fun rules => FV.fvDVarSet (rulesFVs rules).
+
+Definition ruleLhsFVIds : CoreSyn.CoreRule -> FV.FV :=
+  fun arg_0__ =>
+    match arg_0__ with
+    | CoreSyn.BuiltinRule _ _ _ _ => FV.emptyFV
+    | CoreSyn.Rule _ _ _ _ bndrs args _ _ _ _ _ =>
+        FV.filterFV Var.isLocalId (addBndrs bndrs (exprs_fvs args))
+    end.
+
+Definition ruleLhsFreeIds : CoreSyn.CoreRule -> VarSet.VarSet :=
+  FV.fvVarSet GHC.Base.∘ ruleLhsFVIds.
+
+Definition ruleLhsFreeIdsList : CoreSyn.CoreRule -> list Var.Var :=
+  FV.fvVarList GHC.Base.∘ ruleLhsFVIds.
+
+Definition idRuleRhsVars
+   : (BasicTypes.Activation -> bool) -> Var.Id -> VarSet.VarSet :=
+  fun is_active id =>
+    let get_fvs :=
+      fun arg_0__ =>
+        match arg_0__ with
+        | CoreSyn.Rule _ act fn _ bndrs _ rhs _ _ _ _ =>
+            let fvs :=
+              FV.fvVarSet (FV.filterFV Var.isLocalVar (addBndrs bndrs (expr_fvs rhs))) in
+            if is_active act : bool
+            then UniqSet.delOneFromUniqSet_Directly fvs (Unique.getUnique fn) else
+            noFVs
+        | _ => noFVs
+        end in
+    VarSet.emptyVarSet.
+
+Definition rhs_fvs : (Var.Id * CoreSyn.CoreExpr)%type -> FV.FV :=
+  fun '(pair bndr rhs) =>
+    FV.unionFV (expr_fvs rhs) (bndrRuleAndUnfoldingFVs bndr).
+
+Definition bindFreeVars : CoreSyn.CoreBind -> VarSet.VarSet :=
+  fun arg_0__ =>
+    match arg_0__ with
+    | CoreSyn.NonRec b r =>
+        FV.fvVarSet (FV.filterFV Var.isLocalVar (rhs_fvs (pair b r)))
+    | CoreSyn.Rec prs =>
+        FV.fvVarSet (FV.filterFV Var.isLocalVar (addBndrs (GHC.Base.map Data.Tuple.fst
+                                                           prs) (FV.mapUnionFV rhs_fvs prs)))
+    end.
+
+Definition ruleRhsFreeVars : CoreSyn.CoreRule -> VarSet.VarSet :=
+  fun arg_0__ =>
+    match arg_0__ with
+    | CoreSyn.BuiltinRule _ _ _ _ => noFVs
+    | CoreSyn.Rule _ _ _ _ bndrs _ rhs _ _ _ _ =>
+        FV.fvVarSet (FV.filterFV Var.isLocalVar (addBndrs bndrs (expr_fvs rhs)))
+    end.
+
+Definition stableUnfoldingFVs : CoreSyn.Unfolding -> option FV.FV :=
+  fun unf =>
+    let j_1__ :=
+      match unf with
+      | CoreSyn.DFunUnfolding bndrs _ args =>
+          Some (FV.filterFV Var.isLocalVar (FV.delFVs (VarSet.mkVarSet bndrs) (exprs_fvs
+                                                       args)))
+      | _other => None
+      end in
+    match unf with
+    | CoreSyn.CoreUnfolding rhs src _ _ _ _ _ _ =>
+        if CoreSyn.isStableSource src : bool
+        then Some (FV.filterFV Var.isLocalVar (expr_fvs rhs)) else
+        j_1__
+    | _ => j_1__
+    end.
+
+Definition stableUnfoldingVars : CoreSyn.Unfolding -> option VarSet.VarSet :=
+  fun unf => GHC.Base.fmap FV.fvVarSet (stableUnfoldingFVs unf).
+
+Definition vectsFreeVars : list CoreSyn.CoreVect -> VarSet.VarSet :=
+  let vectFreeVars :=
+    fun arg_0__ =>
+      match arg_0__ with
+      | CoreSyn.Vect _ rhs => FV.fvVarSet (FV.filterFV Var.isLocalId (expr_fvs rhs))
+      | CoreSyn.NoVect _ => noFVs
+      | CoreSyn.VectType _ _ _ => noFVs
+      | CoreSyn.VectClass _ => noFVs
+      | CoreSyn.VectInst _ => noFVs
+      end in
+  VarSet.mapUnionVarSet vectFreeVars.
 
 (* External variables:
-     AnnAlt AnnExpr bool list op_zt__ option BasicTypes.Activation CoreSyn.AnnBind
-     CoreSyn.AnnExpr' CoreSyn.CoreBind CoreSyn.CoreBndr CoreSyn.CoreExpr
-     CoreSyn.CoreRule CoreSyn.CoreVect CoreSyn.Unfolding FV.FV FV.InterestingVarFun
-     NameSet.NameSet Var.Id Var.Var VarSet.DIdSet VarSet.DVarSet VarSet.IdSet
-     VarSet.VarSet
+     AnnAlt AnnExpr None Some bool cons freeVarsBind1 list op_zt__ option pair
+     rhs_fvs1 tt BasicTypes.Activation CoreSyn.AnnApp CoreSyn.AnnBind CoreSyn.AnnCase
+     CoreSyn.AnnCast CoreSyn.AnnCoercion CoreSyn.AnnExpr' CoreSyn.AnnLam
+     CoreSyn.AnnLet CoreSyn.AnnLit CoreSyn.AnnNonRec CoreSyn.AnnRec CoreSyn.AnnTick
+     CoreSyn.AnnType CoreSyn.AnnVar CoreSyn.App CoreSyn.Breakpoint
+     CoreSyn.BuiltinRule CoreSyn.Case CoreSyn.Cast CoreSyn.Coercion CoreSyn.CoreBind
+     CoreSyn.CoreBndr CoreSyn.CoreExpr CoreSyn.CoreRule CoreSyn.CoreUnfolding
+     CoreSyn.CoreVect CoreSyn.DFunUnfolding CoreSyn.Lam CoreSyn.Let CoreSyn.Lit
+     CoreSyn.NoVect CoreSyn.NonRec CoreSyn.Rec CoreSyn.Rule CoreSyn.Tick
+     CoreSyn.Tickish CoreSyn.Type_ CoreSyn.Unfolding CoreSyn.Var CoreSyn.Vect
+     CoreSyn.VectClass CoreSyn.VectInst CoreSyn.VectType CoreSyn.isStableSource
+     Data.Foldable.foldr Data.Tuple.fst FV.FV FV.InterestingVarFun FV.delFV FV.delFVs
+     FV.emptyFV FV.filterFV FV.fvDVarSet FV.fvVarList FV.fvVarSet FV.mapUnionFV
+     FV.mkFVs FV.unionFV FV.unitFV GHC.Base.fmap GHC.Base.map GHC.Base.op_z2218U__
+     GHC.DeferredFix.deferredFix4 GHC.List.unzip GHC.List.zip Lists.List.map
+     NameSet.NameSet NameSet.emptyNameSet NameSet.unionNameSet
+     UniqSet.delOneFromUniqSet_Directly Unique.getUnique Var.Id Var.Var Var.isId
+     Var.isLocalId Var.isLocalVar VarSet.DIdSet VarSet.DTyCoVarSet VarSet.DVarSet
+     VarSet.IdSet VarSet.TyCoVarSet VarSet.VarSet VarSet.delDVarSet
+     VarSet.emptyDVarSet VarSet.emptyVarSet VarSet.mapUnionVarSet VarSet.mkDVarSet
+     VarSet.mkVarSet VarSet.unionDVarSet VarSet.unionDVarSets VarSet.unitDVarSet
 *)
