examples/ghc/deps/CoreFVs.mk
@@ -1,1 +1,1 @@
-lib/CoreFVs.v: 
+lib/CoreFVs.v: lib/CoreSyn.h2ci
