examples/ghc/module-edits/CoreFVs/midamble.v
@@ -1,0 +1,14 @@
+(* Break mutual recursion *)
+Parameter rhs_fvs1 : (Var.Id * CoreSyn.CoreExpr)%type -> FV.FV.
+
+(* Break mutual recursion *)
+Parameter freeVarsBind1 : CoreSyn.CoreBind ->
+     VarSet.DVarSet -> (CoreBindWithFVs * VarSet.DVarSet)%type.
+
+(*
+NOTE (freeVars): if you try to use a termination edit for freeVars instead of 
+the rewrite of unzipAndMap in the edit file, we need to add a type
+annotation to fv_alt for the freeVars function to type check. 
+The required annotation is 
+   fv_alt : Alt CoreBndr -> (VarSet.DVarSet * CoreAltWithFVs)
+*)
